goldilocks cleanup
remodularize

src/NewBaseSystem.v
@@ -43,104 +43,30 @@ Require Crypto.Util.Tuple. Local Notation tuple := Tuple.tuple.
       rewrite <-Z.mul_mod, <-Z.add_mod by auto; reflexivity.
     Qed.
 
-Section Goldilocks.
-  Context {s p : Z} {p_nonzero : p <> 0} {s_nonzero : s <> 0}
-          {s2_modp : (s^2) mod p = (s+1) mod p}.
-  Context {T : Type}
-          {eval : T -> Z}
-          {sub : T -> T -> T}
-          {eval_sub : forall x y, eval (sub x y) = eval x - eval y}
-          {mul : T -> T -> T}
-          {eval_mul : forall x y, eval (mul x y) = eval x * eval y}
-          {add : T -> T -> T}
-          {eval_add : forall x y, eval (add x y) = eval x + eval y}
-          {scmul : Z -> T -> T}
-          {eval_scmul : forall c x, eval (scmul c x) = c * eval x}
-          {split : Z -> T -> T * T}
-          {eval_split : forall s x, s <> 0 -> eval (fst (split s x)) + s * (eval (snd (split s x))) = eval x}
-  .
-
-  Definition goldilocks_mul (xs ys : T) : T :=
-    let a_b := split s xs in
-    let c_d := split s ys in
-    let ac := mul (fst a_b) (fst c_d) in
-    (add (add ac (mul (snd a_b) (snd c_d)))
-         (scmul s (sub (mul (add (fst a_b) (snd a_b)) (add (fst c_d) (snd c_d))) ac))).
-
-  Local Existing Instances Z.equiv_modulo_Reflexive RelationClasses.eq_Reflexive Z.equiv_modulo_Symmetric Z.equiv_modulo_Transitive Z.mul_mod_Proper Z.add_mod_Proper Z.modulo_equiv_modulo_Proper.
-  Lemma goldilocks_mul_correct xs ys :
-    (eval (goldilocks_mul xs ys)) mod p = (eval xs * eval ys) mod p.
-  Proof.
-    cbv [goldilocks_mul]; intros.
-    repeat rewrite ?eval_mul, ?eval_add, ?eval_sub, ?eval_scmul.
-    rewrite <-(eval_split s xs), <-(eval_split s ys) by assumption.
-    repeat match goal with
-           | [ H : ?x mod ?m = ?y mod ?m |- _ ] => change (Z.equiv_modulo m x y) in H
-           | [ |- ?x mod ?m = ?y mod ?m ] => change (Z.equiv_modulo m x y)
-           end.
-    ring_simplify.
-    setoid_rewrite s2_modp.
-    apply f_equal2; nsatz.
-  Qed.
-End Goldilocks.
-
-Section Karatsuba.
-  Context {T : Type} (eval : T -> Z)
-          (sub : T -> T -> T)
-          (eval_sub : forall x y, eval (sub x y) = eval x - eval y)
-          (mul : T -> T -> T)
-          (eval_mul : forall x y, eval (mul x y) = eval x * eval y)
-          (add : T -> T -> T)
-          (eval_add : forall x y, eval (add x y) = eval x + eval y)
-          (scmul : Z -> T -> T)
-          (eval_scmul : forall c x, eval (scmul c x) = c * eval x)
-          (split : Z -> T -> T * T)
-          (eval_split : forall s x, s <> 0 -> eval (fst (split s x)) + s * (eval (snd (split s x))) = eval x)
-  .
-
-  Definition karatsuba_mul s (x y : T) : T :=
-      let xab := split s x in
-      let yab := split s y in
-      let xy0 := mul (fst xab) (fst yab) in
-      let xy2 := mul (snd xab) (snd yab) in
-      let xy1 := sub (mul (add (fst xab) (snd xab)) (add (fst yab) (snd yab))) (add xy2 xy0) in
-      add (add (scmul (s^2) xy2) (scmul s xy1)) xy0.
-
-  Lemma eval_karatsuba_mul s x y : s <> 0 ->
-                                   eval (karatsuba_mul s x y) = eval x * eval y.
-  Proof.
-    cbv [karatsuba_mul]; intros.
-    repeat rewrite ?eval_sub, ?eval_mul, ?eval_add, ?eval_scmul.
-    rewrite <-(eval_split s x), <-(eval_split s y) by assumption.
-    ring.
-  Qed.
-
-End Karatsuba.
-
 Delimit Scope runtime_scope with RT.
 Definition runtime_mul := Z.mul. Global Infix "*" := runtime_mul : runtime_scope.
 Definition runtime_add := Z.add. Global Infix "+" := runtime_add : runtime_scope. 
 
 Module B.
   Let limb := (Z*Z)%type. (* position coefficient and run-time value *)
-  Definition eval (p:list limb) : Z :=
-    List.fold_right Z.add 0%Z (List.map (fun t => fst t * snd t) p).
-  
-  Lemma eval_nil : eval nil = 0. Proof. reflexivity. Qed.
-  Lemma eval_cons p q : eval (p::q) = (fst p) * (snd p) + eval q. Proof. reflexivity. Qed.
-  Lemma eval_app p q: eval (p++q) = eval p + eval q.
-  Proof. induction p; simpl eval; rewrite ?eval_nil, ?eval_cons; nsatz. Qed.
+  Module Associational.
+    Definition eval (p:list limb) : Z :=
+      List.fold_right Z.add 0%Z (List.map (fun t => fst t * snd t) p).
+    
+    Lemma eval_nil : eval nil = 0. Proof. reflexivity. Qed.
+    Lemma eval_cons p q : eval (p::q) = (fst p) * (snd p) + eval q. Proof. reflexivity. Qed.
+    Lemma eval_app p q: eval (p++q) = eval p + eval q.
+    Proof. induction p; simpl eval; rewrite ?eval_nil, ?eval_cons; nsatz. Qed.
 
-  Definition mul (p q:list limb) : list limb :=
-    List.flat_map (fun t => List.map (fun t' => (fst t * fst t', (snd t * snd t')%RT)) q) p.
-  Lemma eval_map_mul a x q : eval (List.map (fun t => (a * fst t, x * snd t)) q) = a * x * eval q.
-  Proof. induction q; simpl List.map;
-           rewrite ?eval_nil, ?eval_cons, ?fst_pair, ?snd_pair; nsatz. Qed.
-  Lemma eval_mul p q : eval (mul p q) = eval p * eval q.
-  Proof. induction p; simpl mul;
-           rewrite ?eval_nil, ?eval_cons, ?eval_app, ?eval_map_mul; nsatz. Qed.
+    Definition mul (p q:list limb) : list limb :=
+      List.flat_map (fun t => List.map (fun t' => (fst t * fst t', (snd t * snd t')%RT)) q) p.
+    Lemma eval_map_mul a x q : eval (List.map (fun t => (a * fst t, x * snd t)) q) = a * x * eval q.
+    Proof. induction q; simpl List.map;
+             rewrite ?eval_nil, ?eval_cons, ?fst_pair, ?snd_pair; nsatz. Qed.
+    Lemma eval_mul p q : eval (mul p q) = eval p * eval q.
+    Proof. induction p; simpl mul;
+             rewrite ?eval_nil, ?eval_cons, ?eval_app, ?eval_map_mul; nsatz. Qed.
 
-  Section GeneralizedMersenneReduction.
     Fixpoint split (s:Z) (xs:list limb) : list limb * list limb :=
       match xs with
       | nil => (nil, nil)
@@ -174,80 +100,153 @@ Module B.
       eval (reduce s c p) mod (s - eval c) = eval p mod (s - eval c).
     Proof. cbv [reduce].
            rewrite eval_app, eval_mul, <-reduction_rule, eval_split; trivial. Qed.
-  End GeneralizedMersenneReduction.
+  End Associational.
 
-  Section Positional.
-    Context (weight : nat -> Z) (* [weight i] is the weight of position [i] *)
-            (weight_0 : weight 0%nat = 1%Z)
-            (weight_nonzero : forall i, weight i <> 0).
+  Module Positional.
+    Section Positional.
+      Import Associational.
+      Context (weight : nat -> Z) (* [weight i] is the weight of position [i] *)
+              (weight_0 : weight 0%nat = 1%Z)
+              (weight_nonzero : forall i, weight i <> 0).
 
-    Definition from_positional {n:nat} (xs:tuple Z n) : list limb :=
-      List.combine (List.map weight (List.seq 0 n)) (Tuple.to_list n xs).
+      Definition to_associational {n:nat} (xs:tuple Z n) : list limb :=
+        List.combine (List.map weight (List.seq 0 n)) (Tuple.to_list n xs).
+      Definition eval {n} x := Associational.eval (@to_associational n x).
 
-    Program Definition add_to_nth {n} i x : tuple Z n -> tuple Z n :=
-      Tuple.on_tuple (ListUtil.update_nth i (runtime_add x)) _.
-    Next Obligation. apply ListUtil.length_update_nth. Defined.
+      Program Definition add_to_nth {n} i x : tuple Z n -> tuple Z n :=
+        Tuple.on_tuple (ListUtil.update_nth i (runtime_add x)) _.
+      Next Obligation. apply ListUtil.length_update_nth. Defined.
 
-    Lemma eval_positional_add_to_nth {n} (i:nat) (H:(i<n)%nat) (x:Z) (xs:tuple Z n) :
-      eval (from_positional (add_to_nth i x xs)) = weight i * x + eval (from_positional xs).
-    Proof.
-      cbv [from_positional add_to_nth Tuple.on_tuple]; rewrite !Tuple.to_list_from_list.
-      rewrite ListUtil.combine_update_nth_r at 1.
-      rewrite <-(update_nth_id i (List.combine _ _)) at 2.
-      rewrite <-!(ListUtil.splice_nth_equiv_update_nth_update _ _ (weight 0, 0)) by (autorewrite with distr_length; lia); progress cbv [ListUtil.splice_nth id].
-      repeat match goal with
-             | |- context[?w] => progress (replace w with (weight i); [ring|])
-             | _ => progress rewrite ?eval_app, ?eval_cons, ?fst_pair, ?snd_pair, <-?ListUtil.map_nth_default_always, ?map_fst_combine, ?List.firstn_all2, ?ListUtil.map_nth_default_always, ?nth_default_seq_inbouns, ?(eq_refl:runtime_add=Z.add) by (autorewrite with distr_length; lia)
-             | _ => reflexivity
-             end.
-    Qed.
+      Lemma eval_add_to_nth {n} (i:nat) (H:(i<n)%nat) (x:Z) (xs:tuple Z n) :
+        eval (add_to_nth i x xs) = weight i * x + eval xs.
+      Proof.
+        cbv [eval to_associational add_to_nth Tuple.on_tuple]; rewrite !Tuple.to_list_from_list.
+        rewrite ListUtil.combine_update_nth_r at 1.
+        rewrite <-(update_nth_id i (List.combine _ _)) at 2.
+        rewrite <-!(ListUtil.splice_nth_equiv_update_nth_update _ _ (weight 0, 0)) by (autorewrite with distr_length; lia); progress cbv [ListUtil.splice_nth id].
+        repeat match goal with
+               | _ => progress (apply Zminus_eq; ring_simplify)
+               | _ => progress rewrite ?eval_app, ?eval_cons, ?fst_pair, ?snd_pair, <-?ListUtil.map_nth_default_always, ?map_fst_combine, ?List.firstn_all2, ?ListUtil.map_nth_default_always, ?nth_default_seq_inbouns, ?(eq_refl:runtime_add=Z.add), ?((fun _ => eq_refl):forall x, (0+x=x)%nat) by (autorewrite with distr_length; lia)
+               | _ => solve [trivial]
+               end.
+      Qed.
 
-    Fixpoint place (t:limb) (i:nat) : nat * Z :=
-      if dec (fst t mod weight i = 0)
-      then (i, let c := fst t / weight i in (c * snd t)%RT)
-      else match i with S i' => place t i' | O => (O, fst t * snd t)%RT end.
+      Fixpoint place (t:limb) (i:nat) : nat * Z :=
+        if dec (fst t mod weight i = 0)
+        then (i, let c := fst t / weight i in (c * snd t)%RT)
+        else match i with S i' => place t i' | O => (O, fst t * snd t)%RT end.
 
-    Lemma place_in_range (t:limb) (n:nat) : (fst (place t n) < S n)%nat.
-    Proof. induction n; simpl; break_match; simpl; omega. Qed.
+      Lemma place_in_range (t:limb) (n:nat) : (fst (place t n) < S n)%nat.
+      Proof. induction n; simpl; break_match; simpl; omega. Qed.
 
-    Lemma eval_place t i :
-      weight (fst (place t i)) * snd (place t i) = fst t * snd t.
-    Proof. induction i; simpl place; break_match;
-             try match goal with H:_ |- _ => pose proof (Z_div_exact_full_2 _ _ (weight_nonzero _) H) end;
-             rewrite ?weight_0, ?Z.div_1_r, ?fst_pair, ?snd_pair; nsatz. Qed.
+      Lemma eval_place t i :
+        weight (fst (place t i)) * snd (place t i) = fst t * snd t.
+      Proof. induction i; simpl place; break_match;
+               repeat match goal with H:_ |- _ => unique pose proof (Z_div_exact_full_2 _ _ (weight_nonzero _) H) end;
+               rewrite ?weight_0, ?Z.div_1_r, ?fst_pair, ?snd_pair; nsatz. Qed.
 
-    Definition to_positional {n} (init:tuple Z n) (p:list limb) :=
-      List.fold_right (fun t => let p := place t (pred n) in add_to_nth (fst p) (snd p)) init p.
-    Lemma eval_from_positional_to_positional {n} p (init:tuple Z n) (n_nonzero:n<>O) :
-      eval (from_positional (to_positional init p)) = eval p + eval (from_positional init).
-    Proof. induction p; simpl; try pose proof place_in_range a (pred n);
-             rewrite ?eval_positional_add_to_nth by omega;
-             rewrite ?eval_cons, ?eval_place; try nsatz. Qed.
+      Definition from_associational {n} (init:tuple Z n) (p:list limb) :=
+        List.fold_right (fun t => let p := place t (pred n) in add_to_nth (fst p) (snd p)) init p.
+      Lemma eval_from_associational {n} p (init:tuple Z n) (n_nonzero:n<>O) :
+        eval (from_associational init p) = Associational.eval p + eval init.
+      Proof. induction p; simpl; try pose proof place_in_range a (pred n);
+               rewrite ?eval_add_to_nth by omega;
+               rewrite ?eval_cons, ?eval_place; try nsatz. Qed.
+    End Positional.
   End Positional.
-
 End B.
+
+Section Karatsuba.
+  Context {T : Type} (eval : T -> Z)
+          (sub : T -> T -> T)
+          (eval_sub : forall x y, eval (sub x y) = eval x - eval y)
+          (mul : T -> T -> T)
+          (eval_mul : forall x y, eval (mul x y) = eval x * eval y)
+          (add : T -> T -> T)
+          (eval_add : forall x y, eval (add x y) = eval x + eval y)
+          (scmul : Z -> T -> T)
+          (eval_scmul : forall c x, eval (scmul c x) = c * eval x)
+          (split : Z -> T -> T * T)
+          (eval_split : forall s x, s <> 0 -> eval (fst (split s x)) + s * (eval (snd (split s x))) = eval x)
+  .
+
+  Definition karatsuba_mul s (x y : T) : T :=
+      let xab := split s x in
+      let yab := split s y in
+      let xy0 := mul (fst xab) (fst yab) in
+      let xy2 := mul (snd xab) (snd yab) in
+      let xy1 := sub (mul (add (fst xab) (snd xab)) (add (fst yab) (snd yab))) (add xy2 xy0) in
+      add (add (scmul (s^2) xy2) (scmul s xy1)) xy0.
+
+  Lemma eval_karatsuba_mul s x y : s <> 0 ->
+                                   eval (karatsuba_mul s x y) = eval x * eval y.
+  Proof.
+    cbv [karatsuba_mul]; intros.
+    repeat rewrite ?eval_sub, ?eval_mul, ?eval_add, ?eval_scmul.
+    rewrite <-(eval_split s x), <-(eval_split s y) by assumption.
+    ring.
+  Qed.
+End Karatsuba.
+
+Section Goldilocks.
+  Context {T : Type}
+          (eval : T -> Z)
+          (add : T -> T -> T)
+          (eval_add : forall x y, eval (add x y) = eval x + eval y)
+          (sub : T -> T -> T)
+          (eval_sub : forall x y, eval (sub x y) = eval x - eval y)
+          (mul : T -> T -> T)
+          (eval_mul : forall x y, eval (mul x y) = eval x * eval y)
+          (scmul : Z -> T -> T) (* COMPILE TIME scaling *)
+          (eval_scmul : forall c x, eval (scmul c x) = c * eval x)
+          (split : Z -> T -> T * T)
+          (eval_split : forall s x, eval (fst (split s x)) + s * (eval (snd (split s x))) = eval x)
+  .
+
+  Context (s p : Z) (p_nonzero : p <> 0) (s_nonzero : s <> 0)
+          (s2_modp : (s^2) mod p = (s+1) mod p).
+
+  Definition goldilocks_mul (xs ys : T) : T :=
+    let a_b := split s xs in
+    let c_d := split s ys in
+    let ac := mul (fst a_b) (fst c_d) in
+    (add (add ac (mul (snd a_b) (snd c_d)))
+         (scmul s (sub (mul (add (fst a_b) (snd a_b)) (add (fst c_d) (snd c_d))) ac))).
+
+  Local Existing Instances Z.equiv_modulo_Reflexive RelationClasses.eq_Reflexive Z.equiv_modulo_Symmetric Z.equiv_modulo_Transitive Z.mul_mod_Proper Z.add_mod_Proper Z.modulo_equiv_modulo_Proper.
+
+  Lemma goldilocks_mul_correct xs ys :
+    (eval (goldilocks_mul xs ys)) mod p = (eval xs * eval ys) mod p.
+  Proof.
+    cbv [goldilocks_mul]; Zmod_to_equiv_modulo.
+    repeat rewrite ?eval_mul, ?eval_add, ?eval_sub, ?eval_scmul, <-?(eval_split s xs), <-?(eval_split s ys); ring_simplify.
+    setoid_rewrite s2_modp.
+    apply f_equal2; nsatz.
+  Qed.
+End Goldilocks.
 
 Local Coercion Z.of_nat : nat >-> Z.
 Import Coq.Lists.List.ListNotations. Local Open Scope list_scope.
 Program Definition zeros n : tuple Z n := Tuple.from_list n (List.map (fun _ => 0) (List.seq 0 n)) _.
 Next Obligation. rewrite List.map_length, List.seq_length; reflexivity. Qed.
+Import B.
 
 Goal let base10 i := 10^i in forall f0 f1 f2 f3 g0 g1 g2 g3 : Z, False. intros.
-  let t := constr:(B.to_positional base10 (zeros 7)
-                                   (B.mul
-                                      (B.from_positional base10 (Tuple.from_list _ [f0;f1;f2;f3] eq_refl))
-                                      (B.from_positional base10 (Tuple.from_list _ [g0;g1;g2;g3] eq_refl)))) in
+  let t := constr:(Positional.from_associational base10 (zeros 7)
+                                   (Associational.mul
+                                      (Positional.to_associational base10 (Tuple.from_list _ [f0;f1;f2;f3] eq_refl))
+                                      (Positional.to_associational base10 (Tuple.from_list _ [g0;g1;g2;g3] eq_refl)))) in
   let t := (eval cbv -[runtime_mul runtime_add] in t) in
   let t := (eval cbv [runtime_mul runtime_add] in t) in
   remember t eqn:Heqt; rewrite !Z.mul_1_l, !Z.add_0_r, !Z.add_assoc in Heqt.
 Abort.
 
 Goal let base2_51 i := 2 ^ (51 * i) in forall f0 f1 f2 f3 f4 g0 g1 g2 g3 g4 : Z, False. intros.
-  let t := constr:(B.to_positional base2_51 (zeros 5)
-                                   (B.reduce (2^255) [(1,19)] 
-                                   (B.mul
-                                      (B.from_positional base2_51 (Tuple.from_list _ [f0;f1;f2;f3;f4] eq_refl))
-                                      (B.from_positional base2_51 (Tuple.from_list _ [g0;g1;g2;g3;g4] eq_refl))))) in
+  let t := constr:(Positional.from_associational base2_51 (zeros 5)
+                                   (Associational.reduce (2^255) [(1,19)] 
+                                   (Associational.mul
+                                      (Positional.to_associational base2_51 (Tuple.from_list _ [f0;f1;f2;f3;f4] eq_refl))
+                                      (Positional.to_associational base2_51 (Tuple.from_list _ [g0;g1;g2;g3;g4] eq_refl))))) in
   let t := (eval cbv -[runtime_mul runtime_add] in t) in
   let t := (eval cbv [runtime_mul runtime_add] in t) in
   remember t eqn:Heqt; rewrite !Z.mul_1_l, !Z.add_0_r, !Z.add_assoc, !Z.mul_assoc in Heqt.
@@ -255,63 +254,48 @@ Abort.
 
 
 Goal let base2_25_5 i := 2 ^ (25 * (i / 2) + 26 * (i - i / 2)) in forall f0 f1 f2 f3 f4 f5 f6 f7 f8 f9 g0 g1 g2 g3 g4 g5 g6 g7 g8 g9: Z, False. intros.
-  let t := constr:(B.to_positional base2_25_5 (zeros 10)
-                                   (B.reduce (2^255) [(1,19)] 
-                                   (B.mul
-                                      (B.from_positional base2_25_5 (Tuple.from_list _ [f0;f1;f2;f3;f4;f5;f6;f7;f8;f9] eq_refl))
-                                      (B.from_positional base2_25_5 (Tuple.from_list _ [g0;g1;g2;g3;g4;g5;g6;g7;g8;g9] eq_refl))))) in
+  let t := constr:(Positional.from_associational base2_25_5 (zeros 10)
+                                   (Associational.reduce (2^255) [(1,19)] 
+                                   (Associational.mul
+                                      (Positional.to_associational base2_25_5 (Tuple.from_list _ [f0;f1;f2;f3;f4;f5;f6;f7;f8;f9] eq_refl))
+                                      (Positional.to_associational base2_25_5 (Tuple.from_list _ [g0;g1;g2;g3;g4;g5;g6;g7;g8;g9] eq_refl))))) in
   let t := (eval cbv -[runtime_mul runtime_add] in t) in
   let t := (eval cbv [runtime_mul runtime_add] in t) in
   remember t eqn:Heqt; rewrite !Z.mul_1_l, !Z.add_0_r, !Z.add_assoc, !Z.mul_assoc in Heqt.
 Abort.
 
 Goal let base2_56 i := 2 ^ (56 * i) in forall f0 f1 f2 f3 f4 f5 f6 f7 g0 g1 g2 g3 g4 g5 g6 g7: Z, False. intros.
-  let t := constr:(B.to_positional base2_56 (zeros 8)
-                                   (B.reduce (2^448) [(2^224,1);(1,-1)] 
-                                   (B.reduce (2^448) [(2^224,1);(1,-1)] 
-                                   (B.mul
-                                      (B.from_positional base2_56 (Tuple.from_list _ [f0;f1;f2;f3;f4;f5;f6;f7] eq_refl))
-                                      (B.from_positional base2_56 (Tuple.from_list _ [g0;g1;g2;g3;g4;g5;g6;g7] eq_refl)))))) in
+  let t := constr:(Positional.from_associational base2_56 (zeros 8)
+                                   (Associational.reduce (2^448) [(2^224,1);(1,-1)] 
+                                   (Associational.reduce (2^448) [(2^224,1);(1,-1)] 
+                                   (Associational.mul
+                                      (Positional.to_associational base2_56 (Tuple.from_list _ [f0;f1;f2;f3;f4;f5;f6;f7] eq_refl))
+                                      (Positional.to_associational base2_56 (Tuple.from_list _ [g0;g1;g2;g3;g4;g5;g6;g7] eq_refl)))))) in
   let t := (eval cbv -[runtime_mul runtime_add] in t) in
   let t := (eval cbv [runtime_mul runtime_add] in t) in
   remember t eqn:Heqt; rewrite !Z.mul_1_l, !Z.add_0_r, !Z.add_assoc, !Z.mul_assoc, !Z.mul_opp_l, !Z.add_opp_r in Heqt.
 Abort.
 
-Check (karatsuba_mul (fun x y => x ++ (List.map (fun t => (fst t, -snd t)) y)) B.mul (@List.app _) (fun x => List.map (fun t => (x * fst t, snd t))) B.split (2^102)).
-Print karatsuba_mul.
-About B.split.
-Require Import Crypto.Algebra.
-Goal let base2_51 i := 2 ^ (51 * i) in forall f0 f1 f2 f3 f4 g0 g1 g2 g3 g4 : Z, False. intros.
-  let t := constr:(B.to_positional base2_51 (zeros 5)
-                                   (B.reduce (2^255) [(1,19)] 
-                                   (karatsuba_mul (fun x y => x ++ (List.map (fun t => (fst t, (-1 * snd t)%RT)) y)) B.mul (@List.app _) (fun x => List.map (fun t => (x * fst t, snd t))) B.split (2^102)                                      (B.from_positional base2_51 (Tuple.from_list _ [f0;f1;f2;f3;f4] eq_refl))
-                                      (B.from_positional base2_51 (Tuple.from_list _ [g0;g1;g2;g3;g4] eq_refl))))) in
-  let t := (eval cbv -[runtime_mul runtime_add] in t) in
-  let t := (eval cbv [runtime_mul runtime_add] in t) in
-    remember t eqn:Heqt; change (Zneg xH) with (Z.opp 1) in Heqt; (* TODO : make this a lemma *)
-  ring_simplify_subterms_in_all.
-Abort.
-
+Require Import Crypto.Algebra. (* TODO: move ring_simplify_subterms_in_all to a different file? *)
 Goal let base2_25_5 i := 2 ^ (25 * (i / 2) + 26 * (i - i / 2)) in forall f0 f1 f2 f3 f4 f5 f6 f7 f8 f9 g0 g1 g2 g3 g4 g5 g6 g7 g8 g9: Z, False. intros.
-  let t := constr:(B.to_positional base2_25_5 (zeros 10)
-                                   (B.reduce (2^255) [(1,19)] 
-                                   (karatsuba_mul (fun x y => x ++ (List.map (fun t => (fst t, (-1 * snd t)%RT)) y)) B.mul (@List.app _) (fun x => List.map (fun t => (x * fst t, snd t))) B.split (2^102)
-                                      (B.from_positional base2_25_5 (Tuple.from_list _ [f0;f1;f2;f3;f4;f5;f6;f7;f8;f9] eq_refl))
-                                      (B.from_positional base2_25_5 (Tuple.from_list _ [g0;g1;g2;g3;g4;g5;g6;g7;g8;g9] eq_refl))))) in
+  let t := constr:(Positional.from_associational base2_25_5 (zeros 10)
+                                   (Associational.reduce (2^255) [(1,19)] 
+                                   (karatsuba_mul (fun x y => x ++ (List.map (fun t => (fst t, (-1 * snd t)%RT)) y)) Associational.mul (@List.app _) (fun x => List.map (fun t => (x * fst t, snd t))) Associational.split (2^102)
+                                      (Positional.to_associational base2_25_5 (Tuple.from_list _ [f0;f1;f2;f3;f4;f5;f6;f7;f8;f9] eq_refl))
+                                      (Positional.to_associational base2_25_5 (Tuple.from_list _ [g0;g1;g2;g3;g4;g5;g6;g7;g8;g9] eq_refl))))) in
   let t := (eval cbv -[runtime_mul runtime_add] in t) in
   let t := (eval cbv [runtime_mul runtime_add] in t) in
   remember t eqn:Heqt; change (Zneg xH) with (Z.opp 1) in Heqt; (* TODO : make this a lemma *)
     ring_simplify_subterms_in_all.
-
 Abort.
 
 Goal let base2_56 i := 2 ^ (56 * i) in forall f0 f1 f2 f3 f4 f5 f6 f7 g0 g1 g2 g3 g4 g5 g6 g7: Z, False. intros.
-  let t := constr:(B.to_positional base2_56 (zeros 8)
-                                   (B.reduce (2^448) [(2^224,1);(1,-1)] 
-                                   (B.reduce (2^448) [(2^224,1);(1,-1)] 
-                                   (B.goldilocks_mul (s:=2^224)
-                                      (B.from_positional base2_56 (Tuple.from_list _ [f0;f1;f2;f3;f4;f5;f6;f7] eq_refl))
-                                      (B.from_positional base2_56 (Tuple.from_list _ [g0;g1;g2;g3;g4;g5;g6;g7] eq_refl)))))) in
+  let t := constr:(Positional.from_associational base2_56 (zeros 8)
+                                   (Associational.reduce (2^448) [(2^224,1);(1,-1)] 
+                                   (Associational.reduce (2^448) [(2^224,1);(1,-1)] 
+                                   (goldilocks_mul (fun x y => x ++ (List.map (fun t => (fst t, (-1 * snd t)%RT)) y)) Associational.mul (@List.app _) (fun x => List.map (fun t => (x * fst t, snd t))) Associational.split (2^224)
+                                      (Positional.to_associational base2_56 (Tuple.from_list _ [f0;f1;f2;f3;f4;f5;f6;f7] eq_refl))
+                                      (Positional.to_associational base2_56 (Tuple.from_list _ [g0;g1;g2;g3;g4;g5;g6;g7] eq_refl)))))) in
   let t := (eval cbv -[runtime_mul runtime_add] in t) in
   let t := (eval cbv [runtime_mul runtime_add] in t) in
   remember t eqn:Heqt; rewrite !Z.mul_1_l, !Z.add_0_r, !Z.add_assoc, !Z.mul_assoc, !Z.mul_opp_l, !Z.add_opp_r, !Z.sub_opp_r in Heqt.
